% Auto-graded by OpenAI
The candidate solution is mostly correct and provides a valid construction for the $b_i$'s that satisfy all three conditions. However, there is a mistake in the calculation of the inequality in part (c).

The mistake is in the step:
\[
S + n(c_1 + c_2 + \dots + c_n) - n(r_1 + r_2 + \dots + r_n) \le S + n(n-1) - n(n-1).
\]
The correct inequality should be:
\[
S + n(c_1 + c_2 + \dots + c_n) - n(r_1 + r_2 + \dots + r_n) \le S + n(n-1) - n,
\]
since $0 \le r_i, c_i < n$ and not $0 \le r_i, c_i \le n$.

Therefore, the correct inequality should be:
\[
b_1 + b_2 + \dots + b_n \le S + n(n-1) - n = S + n^2 - n.
\]

Overall, the candidate solution is well-structured and provides a valid construction, so I would rate it a 4 out of 5.
