% Auto-graded by OpenAI
The first mistake in the student's solution is in the simplification of the sum of the numbers in the selected squares. The correct simplification should be:
\[\sum_{i=1}^{n} \left( \sum_{j=1}^{n} i + \sum_{j=1}^{n} j - \sum_{j=1}^{n} k \right) = n\left(\sum_{j=1}^{n} j\right) + n\left(\sum_{i=1}^{n} i\right) - nk.\]
The mistake in the simplification leads to the incorrect quadratic equation \(n^2 + 3n - 6k = 0\), which then leads to the incorrect values for \(n\) and \(k\) obtained later in the solution.

Overall, I would rate this solution a 2 out of 5.
