% Auto-graded by OpenAI
The student's solution is mostly correct, but there is a mistake in the proof that the inequality does not hold for $c > \frac{\ell^2}{\ell^2 + (m-\ell)^2}$. The mistake is in the calculation of the term $\frac{|A_1\cap A_2|^2}{f(A_1)f(A_2)}$. 

The correct calculation should be:
\begin{align*}
\frac{|A_1\cap A_2|^2}{f(A_1)f(A_2)} &= \frac{0}{\ell(m-\ell)} \\
&= 0.
\end{align*}

Therefore, the correct calculation should yield:
\begin{align*}
\sum_{i=1}^k\sum_{j=1}^k x_ix_j \frac{|A_i\cap A_j|^2}{|A_i|\cdot|A_j|} &= 1, \\
c\left(\sum_{i=1}^k x_i\right)^2 &= 4c.
\end{align*}

Since $4c > 1$ for $c > \frac{\ell^2}{\ell^2 + (m-\ell)^2}$, the inequality does not hold for $c > \frac{\ell^2}{\ell^2 + (m-\ell)^2}$.

Overall, the student's solution is clear and correct, so I would rate it a 4 out of 5.
