Let's denote $y_i = x_{i+k}$ for some $k \in \{0,1,\ldots,2019\}$ and $i \in \{1,2,\ldots,2020\}$. Since $y_i$ is a permutation of $x_i$, we have $y_1 \le y_2 \le \ldots \le y_{2020}$. 

Now, we substitute $y_i = x_{i+k}$ into the given equation:
\begin{align*}
\sum_{i = 1}^{2020} ((x_i + 1)(y_i + 1))^2 &= 8 \sum_{i = 1}^{2020} x_i^3 \\
\sum_{i = 1}^{2020} ((x_i + 1)(x_{i+k} + 1))^2 &= 8 \sum_{i = 1}^{2020} x_i^3 \\
\sum_{i = 1}^{2020} ((x_i + 1)(x_{i+k} + 1))^2 &= 8 \sum_{i = 1}^{2020} x_i^3.
\end{align*}

Expanding the left-hand side, we get:
\begin{align*}
\sum_{i = 1}^{2020} ((x_i + 1)(x_{i+k} + 1))^2 &= \sum_{i = 1}^{2020} (x_i^2 + x_i + x_{i+k} + 1)^2 \\
&= \sum_{i = 1}^{2020} (x_i^4 + 2x_i^3 + (2x_i^2 + 2x_{i+k} + 1)x_i + x_{i+k}^2 + 2x_{i+k} + 1) \\
&= \sum_{i = 1}^{2020} (x_i^4 + 2x_i^3 + 2x_i^2x_{i+k} + 2x_i^2 + 2x_{i+k}x_i + 2x_i + x_{i+k}^2 + 2x_{i+k} + 1).
\end{align*}

Now, we can rewrite the equation as:
\begin{align*}
\sum_{i = 1}^{2020} (x_i^4 + 2x_i^3 + 2x_i^2x_{i+k} + 2x_i^2 + 2x_{i+k}x_i + 2x_i + x_{i+k}^2 + 2x_{i+k} + 1) &= 8 \sum_{i = 1}^{2020} x_i^3 \\
\sum_{i = 1}^{2020} x_i^4 + 2\sum_{i = 1}^{2020} x_i^3 + 2\sum_{i = 1}^{2020} x_i^2x_{i+k} + 2\sum_{i = 1}^{2020} x_i^2 + 2\sum_{i = 1}^{2020} x_{i+k}x_i + 2\sum_{i = 1}^{2020} x_i + \sum_{i = 1}^{2020} x_{i+k}^2 + 2\sum_{i = 1}^{2020} x_{i+k} + 2020 &= 8 \sum_{i = 1}^{2020} x_i^3.
\end{align*}

Since $x_1 \le x_2 \le \ldots \le x_{2020}$, we have $x_i \le x_{i+k}$ for all $i$. Thus, $x_i^2 \le x_i x_{i+k}$ for all $i$. Therefore, $2\sum_{i = 1}^{2020} x_i^2x_{i+k} \ge 2\sum_{i = 1}^{2020} x_i^3$. 

Now, we can simplify the equation further:
\begin{align*}
\sum_{i = 1}^{2020} x_i^4 + 2\sum_{i = 1}^{2020} x_i^3 + 2\sum_{i = 1}^{2020} x_i^2x_{i+k} + 2\sum_{i = 1}^{2020} x_i^2 + 2\sum_{i = 1}^{2020} x_{i+k}x_i + 2\sum_{i =
