From the given equations, we have
\begin{align*}
a^2b + c &= b^2c + a, \\
c^2a + b &= b^2c + a.
\end{align*}
Subtracting the second equation from the first, we get
\[
a^2b - c^2a = 0 \quad \Rightarrow \quad a(ab - c^2) = 0.
\]
Since \(a \neq 0\), we must have \(ab = c^2\). Similarly, subtracting the first equation from the second, we get
\[
c^2a - a^2b = 0 \quad \Rightarrow \quad a(c^2 - ab) = 0.
\]
Since \(a \neq 0\), we must have \(c^2 = ab\). Thus, we have \(ab = c^2 = a^2b\), which implies that \(a = b = c\) or \(a = b = 0\). 

If \(a = b = c\), then substituting this into the first equation \(ab + bc + ca = 1\), we get \(3a^2 = 1\), which gives \(a = b = c = \pm \frac{1}{\sqrt{3}}\).

If \(a = b = 0\), then the first equation \(ab + bc + ca = 1\) gives \(bc = 1\), which is not possible since \(b = 0\).

Therefore, the only solutions are \(a = b = c = \pm \frac{1}{\sqrt{3}}\).
