Let's denote $S$ as the given sum:
\[
S = \sum_{k=0}^{3^{1010}-1} (-2)^{f(k)} (z+k)^{2023}.
\]
Since $f(k)$ counts the number of ones in the base 3 representation of $k$, we know that $f(k)$ can take values from $0$ to $2023$ inclusive. For $f(k) = 0$, we have $(-2)^0 = 1$, and for $f(k) = 1$, we have $(-2)^1 = -2$. Therefore, we can rewrite the sum as follows:
\[
S = \sum_{k=0}^{3^{1010}-1} (z+k)^{2023} - 2\sum_{k=0}^{3^{1010}-1} (z+k)^{2023}.
\]
Now, we will evaluate the two sums separately. 

For the first sum, we have:
\begin{align*}
\sum_{k=0}^{3^{1010}-1} (z+k)^{2023} &= \sum_{k=0}^{3^{1010}-1} k^{2023} + z^{2023} + \sum_{k=0}^{3^{1010}-1} \binom{2023}{1} k^{2022} z + \ldots + \binom{2023}{2022} z^{2022} + \binom{2023}{2023} z^{2023} \\
&= \frac{(3^{1010}-1)(3^{1010})}{2} + (3^{1010})^{2023} + \binom{2023}{1} \frac{(3^{1010}-1)(3^{1010})}{2} z + \ldots + \binom{2023}{2022} \frac{(3^{1010}-1)(3^{1010})}{2} z^{2022} + \binom{2023}{2023} z^{2023} \\
&= \frac{3^{2020}-3^{1010}}{2} + 3^{3030} + \frac{2023 \cdot 3^{2020} - 2023 \cdot 3^{1010}}{2}z + \ldots + \frac{2023!}{2022! \cdot 1!} \cdot \frac{3^{2020}-3^{1010}}{2} z^{2022} + z^{2023} \\
&= \frac{3^{2020}-3^{1010}}{2} + 3^{3030} + \frac{2023 \cdot 3^{2020} - 2023 \cdot 3^{1010}}{2}z + \ldots + 2023 \cdot 3^{2020} z^{2022} + z^{2023}.
\end{align*}

For the second sum, we have:
\begin{align*}
\sum_{k=0}^{3^{1010}-1} (z+k)^{2023} &= \sum_{k=0}^{3^{1010}-1} (-2)(z+k)^{2023} \\
&= -2\left(\frac{3^{2020}-3^{1010}}{2} + 3^{3030} + \frac{2023 \cdot 3^{2020} - 2023 \cdot 3^{1010}}{2}z + \ldots + 2023 \cdot 3^{2020} z^{2022} + z^{2023}\right).
\end{align*}

Therefore, the sum $S$ simplifies to:
\[
S = \frac{3^{2020}-3^{1010}}{2} + 3^{3030} + \frac{2023 \cdot 3^{2020} - 2023 \cdot 3^{1010}}{2}z + \ldots + 2023 \cdot 3^{2020} z^{2022} + z^{2023} - 2\left(\frac{3^{2020}-3^{1010}}{2} + 3^{3030} + \frac{2023 \cdot 3^{2020} - 2023 \cdot 3^{1010}}{2}z + \ldots + 2023 \cdot 3^{2020} z^{2022} + z^{2023}\right).
\]

Simplifying further, we get:
\[
S = \frac{3^{2020}-3^{1010}}{2} + 3^{3030} +
