Let's first consider the given equation modulo 2. Since the left-hand side is even, the right-hand side must also be even. This implies that \( c \) is even. Let \( c = 2k \) for some positive integer \( k \).

Substitute \( c = 2k \) into the given equation:
\[2a^n + 3b^n = 4(2k)^n.\]

Dividing both sides by 2, we get:
\[a^n + \frac{3}{2}b^n = 2^{2n-1}k^n.\]

Now, consider the equation modulo 3. Since the left-hand side is divisible by 3, the right-hand side must also be divisible by 3. This implies that \( k \) is divisible by 3. Let \( k = 3m \) for some positive integer \( m \).

Substitute \( k = 3m \) into the equation:
\[a^n + \frac{3}{2}b^n = 2^{2n-1}(3m)^n.\]

Dividing both sides by 3, we get:
\[\frac{1}{3}a^n + \frac{1}{2}b^n = 2^{2n-2}m^n.\]

Now, consider the equation modulo 2 again. Since the left-hand side is odd, the right-hand side must also be odd. This implies that \( m \) is odd. Let \( m = 2r + 1 \) for some positive integer \( r \).

Substitute \( m = 2r + 1 \) into the equation:
\[\frac{1}{3}a^n + \frac{1}{2}b^n = 2^{2n-2}(2r+1)^n.\]

Multiplying both sides by 6 to clear the fractions, we get:
\[2a^n + 3b^n = 6 \cdot 2^{2n-2}(2r+1)^n.\]

This equation is equivalent to the original equation. Therefore, we have shown that if there exist positive integers \( a \), \( b \), and \( c \) satisfying the original equation, then there exist positive integers \( a \), \( b \), and \( c \) satisfying the equation above.

Now, we can repeat the process of considering the equation modulo 2, 3, and so on, to show that there exist positive integers \( a \), \( b \), and \( c \) satisfying the original equation if and only if there exist positive integers \( a \), \( b \), and \( c \) satisfying the equation
\[2a^n + 3b^n = 6 \cdot 2^{2n-2}(2r+1)^n.\]

Since the equation above is in the form of \(2^x \cdot 3^y = 6 \cdot 2^z \cdot 3^w\), we must have \(x = z\) and \(y = w\). This gives us \(n = 2n-2\), which simplifies to \(n = 2\).

Therefore, the only positive integer \( n \) for which there exist positive integers \( a \), \( b \), and \( c \) satisfying the original equation is \( n = 2 \).
